merge in blocking_semantics

examples/hoare_logic/blocking_semantics3/blocking_semantics3_WP_progress_1.v
@@ -4,6 +4,7 @@ Require Import BuiltIn.
 Require BuiltIn.
 Require int.Int.
 Require int.MinMax.
+Require set.Set.
 
 (* Why3 assumption *)
 Inductive list (a:Type) {a_WT:WhyType a} :=
@@ -13,6 +14,53 @@ Axiom list_WhyType : forall (a:Type) {a_WT:WhyType a}, WhyType (list a).
 Existing Instance list_WhyType.
 Implicit Arguments Nil [[a] [a_WT]].
 Implicit Arguments Cons [[a] [a_WT]].
+
+(* Why3 assumption *)
+Fixpoint infix_plpl {a:Type} {a_WT:WhyType a}(l1:(list a)) (l2:(list
+  a)) {struct l1}: (list a) :=
+  match l1 with
+  | Nil => l2
+  | (Cons x1 r1) => (Cons x1 (infix_plpl r1 l2))
+  end.
+
+Axiom Append_assoc : forall {a:Type} {a_WT:WhyType a}, forall (l1:(list a))
+  (l2:(list a)) (l3:(list a)), ((infix_plpl l1 (infix_plpl l2
+  l3)) = (infix_plpl (infix_plpl l1 l2) l3)).
+
+Axiom Append_l_nil : forall {a:Type} {a_WT:WhyType a}, forall (l:(list a)),
+  ((infix_plpl l (Nil :(list a))) = l).
+
+(* Why3 assumption *)
+Fixpoint length {a:Type} {a_WT:WhyType a}(l:(list a)) {struct l}: Z :=
+  match l with
+  | Nil => 0%Z
+  | (Cons _ r) => (1%Z + (length r))%Z
+  end.
+
+Axiom Length_nonnegative : forall {a:Type} {a_WT:WhyType a}, forall (l:(list
+  a)), (0%Z <= (length l))%Z.
+
+Axiom Length_nil : forall {a:Type} {a_WT:WhyType a}, forall (l:(list a)),
+  ((length l) = 0%Z) <-> (l = (Nil :(list a))).
+
+Axiom Append_length : forall {a:Type} {a_WT:WhyType a}, forall (l1:(list a))
+  (l2:(list a)), ((length (infix_plpl l1
+  l2)) = ((length l1) + (length l2))%Z).
+
+(* Why3 assumption *)
+Fixpoint mem {a:Type} {a_WT:WhyType a}(x:a) (l:(list a)) {struct l}: Prop :=
+  match l with
+  | Nil => False
+  | (Cons y r) => (x = y) \/ (mem x r)
+  end.
+
+Axiom mem_append : forall {a:Type} {a_WT:WhyType a}, forall (x:a) (l1:(list
+  a)) (l2:(list a)), (mem x (infix_plpl l1 l2)) <-> ((mem x l1) \/ (mem x
+  l2)).
+
+Axiom mem_decomp : forall {a:Type} {a_WT:WhyType a}, forall (x:a) (l:(list
+  a)), (mem x l) -> exists l1:(list a), exists l2:(list a),
+  (l = (infix_plpl l1 (Cons x l2))).
 
 Axiom map : forall (a:Type) {a_WT:WhyType a} (b:Type) {b_WT:WhyType b}, Type.
 Parameter map_WhyType : forall (a:Type) {a_WT:WhyType a}
@@ -68,6 +116,9 @@ Axiom mident : Type.
 Parameter mident_WhyType : WhyType mident.
 Existing Instance mident_WhyType.
 
+Axiom mident_decide : forall (m1:mident) (m2:mident), (m1 = m2) \/
+  ~ (m1 = m2).
+
 (* Why3 assumption *)
 Inductive ident  :=
   | mk_ident : Z -> ident .
@@ -79,66 +130,25 @@ Definition ident_index(v:ident): Z := match v with
   | (mk_ident x) => x
   end.
 
+Axiom ident_decide : forall (m1:ident) (m2:ident), (m1 = m2) \/ ~ (m1 = m2).
+
 (* Why3 assumption *)
-Inductive term_node  :=
-  | Tvalue : value -> term_node 
-  | Tvar : ident -> term_node 
-  | Tderef : mident -> term_node 
-  | Tbin : term -> operator -> term -> term_node 
-  with term  :=
-  | mk_term : term_node -> Z -> term .
+Inductive term  :=
+  | Tvalue : value -> term 
+  | Tvar : ident -> term 
+  | Tderef : mident -> term 
+  | Tbin : term -> operator -> term -> term .
 Axiom term_WhyType : WhyType term.
 Existing Instance term_WhyType.
-
-Axiom term_node_WhyType : WhyType term_node.
-Existing Instance term_node_WhyType.
-
-(* Why3 assumption *)
-Definition term_maxvar(v:term): Z := match v with
-  | (mk_term x x1) => x1
-  end.
-
-(* Why3 assumption *)
-Definition term_node1(v:term): term_node :=
-  match v with
-  | (mk_term x x1) => x
-  end.
 
 (* Why3 assumption *)
 Fixpoint var_occurs_in_term(x:ident) (t:term) {struct t}: Prop :=
   match t with
-  | (mk_term (Tvalue _) _) => False
-  | (mk_term (Tvar i) _) => (x = i)
-  | (mk_term (Tderef _) _) => False
-  | (mk_term (Tbin t1 _ t2) _) => (var_occurs_in_term x t1) \/
-      (var_occurs_in_term x t2)
+  | (Tvalue _) => False
+  | (Tvar i) => (x = i)
+  | (Tderef _) => False
+  | (Tbin t1 _ t2) => (var_occurs_in_term x t1) \/ (var_occurs_in_term x t2)
   end.
-
-(* Why3 assumption *)
-Definition term_inv(t:term): Prop := forall (x:ident), (var_occurs_in_term x
-  t) -> ((ident_index x) <= (term_maxvar t))%Z.
-
-(* Why3 assumption *)
-Definition mk_tvalue(v:value): term := (mk_term (Tvalue v) (-1%Z)%Z).
-
-Axiom mk_tvalue_inv : forall (v:value), (term_inv (mk_tvalue v)).
-
-(* Why3 assumption *)
-Definition mk_tvar(i:ident): term := (mk_term (Tvar i) (ident_index i)).
-
-Axiom mk_tvar_inv : forall (i:ident), (term_inv (mk_tvar i)).
-
-(* Why3 assumption *)
-Definition mk_tderef(r:mident): term := (mk_term (Tderef r) (-1%Z)%Z).
-
-Axiom mk_tderef_inv : forall (r:mident), (term_inv (mk_tderef r)).
-
-(* Why3 assumption *)
-Definition mk_tbin(t1:term) (o:operator) (t2:term): term := (mk_term (Tbin t1
-  o t2) (Zmax (term_maxvar t1) (term_maxvar t2))).
-
-Axiom mk_tbin_inv : forall (t1:term) (t2:term) (o:operator),
-  ((term_inv t1) /\ (term_inv t2)) -> (term_inv (mk_tbin t1 o t2)).
 
 (* Why3 assumption *)
 Inductive fmla  :=
@@ -199,19 +209,19 @@ Definition type_env  := (map mident datatype).
 Inductive type_term : (map mident datatype) -> (list (ident* datatype)%type)
   -> term -> datatype -> Prop :=
   | Type_value : forall (sigma:(map mident datatype)) (pi:(list (ident*
-      datatype)%type)) (v:value) (m:Z), (type_term sigma pi
-      (mk_term (Tvalue v) m) (type_value v))
+      datatype)%type)) (v:value), (type_term sigma pi (Tvalue v)
+      (type_value v))
   | Type_var : forall (sigma:(map mident datatype)) (pi:(list (ident*
-      datatype)%type)) (v:ident) (m:Z) (ty:datatype), ((get_vartype v
-      pi) = ty) -> (type_term sigma pi (mk_term (Tvar v) m) ty)
+      datatype)%type)) (v:ident) (ty:datatype), ((get_vartype v pi) = ty) ->
+      (type_term sigma pi (Tvar v) ty)
   | Type_deref : forall (sigma:(map mident datatype)) (pi:(list (ident*
-      datatype)%type)) (v:mident) (m:Z) (ty:datatype), ((get sigma
-      v) = ty) -> (type_term sigma pi (mk_term (Tderef v) m) ty)
+      datatype)%type)) (v:mident) (ty:datatype), ((get sigma v) = ty) ->
+      (type_term sigma pi (Tderef v) ty)
   | Type_bin : forall (sigma:(map mident datatype)) (pi:(list (ident*
-      datatype)%type)) (t1:term) (t2:term) (op:operator) (m:Z) (ty1:datatype)
+      datatype)%type)) (t1:term) (t2:term) (op:operator) (ty1:datatype)
       (ty2:datatype) (ty:datatype), (type_term sigma pi t1 ty1) ->
       ((type_term sigma pi t2 ty2) -> ((type_operator op ty1 ty2 ty) ->
-      (type_term sigma pi (mk_term (Tbin t1 op t2) m) ty))).
+      (type_term sigma pi (Tbin t1 op t2) ty))).
 
 (* Why3 assumption *)
 Inductive type_fmla : (map mident datatype) -> (list (ident* datatype)%type)
@@ -307,17 +317,39 @@ Axiom eval_bin_def : forall (x:value) (op:operator) (y:value), match (x,
 Fixpoint eval_term(sigma:(map mident value)) (pi:(list (ident* value)%type))
   (t:term) {struct t}: value :=
   match t with
-  | (mk_term (Tvalue v) _) => v
-  | (mk_term (Tvar id) _) => (get_stack id pi)
-  | (mk_term (Tderef id) _) => (get sigma id)
-  | (mk_term (Tbin t1 op t2) _) => (eval_bin (eval_term sigma pi t1) op
-      (eval_term sigma pi t2))
+  | (Tvalue v) => v
+  | (Tvar id) => (get_stack id pi)
+  | (Tderef id) => (get sigma id)
+  | (Tbin t1 op t2) => (eval_bin (eval_term sigma pi t1) op (eval_term sigma
+      pi t2))
   end.
 
-Axiom eval_bool_term : forall (sigma:(map mident value)) (pi:(list (ident*
-  value)%type)) (sigmat:(map mident datatype)) (pit:(list (ident*
-  datatype)%type)) (t:term), (type_term sigmat pit t TYbool) ->
-  exists b:bool, ((eval_term sigma pi t) = (Vbool b)).
+(* Why3 assumption *)
+Inductive compatible : datatype -> value -> Prop :=
+  | Compatible_bool : forall (b:bool), (compatible TYbool (Vbool b))
+  | Compatible_int : forall (n:Z), (compatible TYint (Vint n))
+  | Compatible_void : (compatible TYunit Vvoid).
+
+(* Why3 assumption *)
+Definition existe_compatible(ty:datatype) (v:value): Prop :=
+  match ty with
+  | TYbool => exists b:bool, (v = (Vbool b))
+  | TYint => exists n:Z, (v = (Vint n))
+  | TYunit => (v = Vvoid)
+  end.
+
+(* Why3 assumption *)
+Definition compatible_env(sigma:(map mident value)) (sigmat:(map mident
+  datatype)) (pi:(list (ident* value)%type)) (pit:(list (ident*
+  datatype)%type)): Prop := (forall (id:mident), (compatible (get sigmat id)
+  (get sigma id))) /\ forall (id:ident), (compatible (get_vartype id pit)
+  (get_stack id pi)).
+
+Axiom eval_type_term : forall (t:term) (sigma:(map mident value)) (pi:(list
+  (ident* value)%type)) (sigmat:(map mident datatype)) (pit:(list (ident*
+  datatype)%type)) (ty:datatype), (compatible_env sigma sigmat pi pit) ->
+  ((type_term sigmat pit t ty) -> (existe_compatible ty (eval_term sigma pi
+  t))).
 
 (* Why3 assumption *)
 Fixpoint eval_fmla(sigma:(map mident value)) (pi:(list (ident* value)%type))
@@ -340,41 +372,31 @@ Parameter msubst_term: term -> mident -> ident -> term.
 
 Axiom msubst_term_def : forall (t:term) (r:mident) (v:ident),
   match t with
-  | (mk_term ((Tvalue _)|(Tvar _)) _) => ((msubst_term t r v) = t)
-  | (mk_term (Tderef x) _) => ((r = x) -> ((msubst_term t r
-      v) = (mk_tvar v))) /\ ((~ (r = x)) -> ((msubst_term t r v) = t))
-  | (mk_term (Tbin t1 op t2) _) => ((msubst_term t r
-      v) = (mk_tbin (msubst_term t1 r v) op (msubst_term t2 r v)))
+  | ((Tvalue _)|(Tvar _)) => ((msubst_term t r v) = t)
+  | (Tderef x) => ((r = x) -> ((msubst_term t r v) = (Tvar v))) /\
+      ((~ (r = x)) -> ((msubst_term t r v) = t))
+  | (Tbin t1 op t2) => ((msubst_term t r v) = (Tbin (msubst_term t1 r v) op
+      (msubst_term t2 r v)))
   end.
 
 Parameter subst_term: term -> ident -> ident -> term.
 
 Axiom subst_term_def : forall (t:term) (r:ident) (v:ident),
   match t with
-  | (mk_term ((Tvalue _)|(Tderef _)) _) => ((subst_term t r v) = t)
-  | (mk_term (Tvar x) _) => ((r = x) -> ((subst_term t r
-      v) = (mk_tvar v))) /\ ((~ (r = x)) -> ((subst_term t r v) = t))
-  | (mk_term (Tbin t1 op t2) _) => ((subst_term t r
-      v) = (mk_tbin (subst_term t1 r v) op (subst_term t2 r v)))
+  | ((Tvalue _)|(Tderef _)) => ((subst_term t r v) = t)
+  | (Tvar x) => ((r = x) -> ((subst_term t r v) = (Tvar v))) /\
+      ((~ (r = x)) -> ((subst_term t r v) = t))
+  | (Tbin t1 op t2) => ((subst_term t r v) = (Tbin (subst_term t1 r v) op
+      (subst_term t2 r v)))
   end.
 
 (* Why3 assumption *)
-Definition fresh_in_term(id:ident) (t:term): Prop :=
-  ((term_maxvar t) < (ident_index id))%Z.
+Definition fresh_in_term(id:ident) (t:term): Prop := ~ (var_occurs_in_term id
+  t).
 
-Axiom eval_msubst_term : forall (sigma:(map mident value)) (pi:(list (ident*
-  value)%type)) (e:term) (x:mident) (v:ident), (fresh_in_term v e) ->
-  ((eval_term sigma pi (msubst_term e x v)) = (eval_term (set sigma x
-  (get_stack v pi)) pi e)).
-
-Axiom eval_subst_term : forall (sigma:(map mident value)) (pi:(list (ident*
-  value)%type)) (e:term) (x:ident) (v:ident), (fresh_in_term v e) ->
-  ((eval_term sigma pi (subst_term e x v)) = (eval_term sigma (Cons (x,
-  (get_stack v pi)) pi) e)).
-
-Axiom eval_term_change_free : forall (t:term) (sigma:(map mident value))
-  (pi:(list (ident* value)%type)) (id:ident) (v:value), (fresh_in_term id
-  t) -> ((eval_term sigma (Cons (id, v) pi) t) = (eval_term sigma pi t)).
+Axiom fresh_in_binop : forall (t:term) (t':term) (op:operator) (v:ident),
+  (fresh_in_term v (Tbin t op t')) -> ((fresh_in_term v t) /\
+  (fresh_in_term v t')).
 
 (* Why3 assumption *)
 Fixpoint fresh_in_fmla(id:ident) (f:fmla) {struct f}: Prop :=
@@ -410,59 +432,56 @@ Fixpoint msubst(f:fmla) (x:mident) (v:ident) {struct f}: fmla :=
   | (Fforall y ty f1) => (Fforall y ty (msubst f1 x v))
   end.
 
+Axiom subst_fresh_term : forall (t:term) (x:ident) (v:ident),
+  (fresh_in_term x t) -> ((subst_term t x v) = t).
+
 Axiom subst_fresh : forall (f:fmla) (x:ident) (v:ident), (fresh_in_fmla x
   f) -> ((subst f x v) = f).
 
-Axiom let_subst : forall (t:term) (f:fmla) (x:ident) (id':ident) (id:mident),
-  ((msubst (Flet x t f) id id') = (Flet x (msubst_term t id id') (msubst f id
-  id'))).
+Axiom eval_msubst_term : forall (e:term) (sigma:(map mident value)) (pi:(list
+  (ident* value)%type)) (x:mident) (v:ident), (fresh_in_term v e) ->
+  ((eval_term sigma pi (msubst_term e x v)) = (eval_term (set sigma x
+  (get_stack v pi)) pi e)).
 
 Axiom eval_msubst : forall (f:fmla) (sigma:(map mident value)) (pi:(list
   (ident* value)%type)) (x:mident) (v:ident), (fresh_in_fmla v f) ->
   ((eval_fmla sigma pi (msubst f x v)) <-> (eval_fmla (set sigma x
   (get_stack v pi)) pi f)).
 
-Axiom eval_subst : forall (f:fmla) (sigma:(map mident value)) (pi:(list
-  (ident* value)%type)) (x:ident) (v:ident), (fresh_in_fmla v f) ->
-  ((eval_fmla sigma pi (subst f x v)) <-> (eval_fmla sigma (Cons (x,
-  (get_stack v pi)) pi) f)).
+Axiom eval_swap_term : forall (t:term) (sigma:(map mident value)) (pi:(list
+  (ident* value)%type)) (l:(list (ident* value)%type)) (id1:ident)
+  (id2:ident) (v1:value) (v2:value), (~ (id1 = id2)) -> ((eval_term sigma
+  (infix_plpl l (Cons (id1, v1) (Cons (id2, v2) pi))) t) = (eval_term sigma
+  (infix_plpl l (Cons (id2, v2) (Cons (id1, v1) pi))) t)).
+
+Axiom eval_swap_term_2 : forall (t:term) (sigma:(map mident value)) (pi:(list
+  (ident* value)%type)) (id1:ident) (id2:ident) (v1:value) (v2:value),
+  (~ (id1 = id2)) -> ((eval_term sigma (Cons (id1, v1) (Cons (id2, v2) pi))
+  t) = (eval_term sigma (Cons (id2, v2) (Cons (id1, v1) pi)) t)).
 
 Axiom eval_swap : forall (f:fmla) (sigma:(map mident value)) (pi:(list
-  (ident* value)%type)) (id1:ident) (id2:ident) (v1:value) (v2:value),
-  (~ (id1 = id2)) -> ((eval_fmla sigma (Cons (id1, v1) (Cons (id2, v2) pi))
-  f) <-> (eval_fmla sigma (Cons (id2, v2) (Cons (id1, v1) pi)) f)).
+  (ident* value)%type)) (l:(list (ident* value)%type)) (id1:ident)
+  (id2:ident) (v1:value) (v2:value), (~ (id1 = id2)) -> ((eval_fmla sigma
+  (infix_plpl l (Cons (id1, v1) (Cons (id2, v2) pi))) f) <-> (eval_fmla sigma
+  (infix_plpl l (Cons (id2, v2) (Cons (id1, v1) pi))) f)).
 
-Axiom eval_same_var : forall (f:fmla) (sigma:(map mident value)) (pi:(list
-  (ident* value)%type)) (id:ident) (v1:value) (v2:value), (eval_fmla sigma
-  (Cons (id, v1) (Cons (id, v2) pi)) f) <-> (eval_fmla sigma (Cons (id, v1)
-  pi) f).
+Axiom eval_swap_2 : forall (f:fmla) (id1:ident) (id2:ident) (v1:value)
+  (v2:value), (~ (id1 = id2)) -> forall (sigma:(map mident value)) (pi:(list
+  (ident* value)%type)), (eval_fmla sigma (Cons (id1, v1) (Cons (id2, v2)
+  pi)) f) <-> (eval_fmla sigma (Cons (id2, v2) (Cons (id1, v1) pi)) f).
 
-Axiom eval_change_free : forall (f:fmla) (sigma:(map mident value)) (pi:(list
-  (ident* value)%type)) (id:ident) (v:value), (fresh_in_fmla id f) ->
-  ((eval_fmla sigma (Cons (id, v) pi) f) <-> (eval_fmla sigma pi f)).
+Axiom eval_term_change_free : forall (t:term) (sigma:(map mident value))
+  (pi:(list (ident* value)%type)) (id:ident) (v:value), (fresh_in_term id
+  t) -> ((eval_term sigma (Cons (id, v) pi) t) = (eval_term sigma pi t)).
+
+Axiom eval_change_free : forall (f:fmla) (id:ident) (v:value),
+  (fresh_in_fmla id f) -> forall (sigma:(map mident value)) (pi:(list (ident*
+  value)%type)), (eval_fmla sigma (Cons (id, v) pi) f) <-> (eval_fmla sigma
+  pi f).
 
 (* Why3 assumption *)
 Definition valid_fmla(p:fmla): Prop := forall (sigma:(map mident value))
   (pi:(list (ident* value)%type)), (eval_fmla sigma pi p).
-
-Axiom msubst_implies : forall (p:fmla) (q:fmla), (valid_fmla (Fimplies p
-  q)) -> forall (sigma:(map mident value)) (pi:(list (ident* value)%type))
-  (x:mident) (id:ident), (fresh_in_fmla id (Fand p q)) -> (eval_fmla sigma
-  (Cons (id, (get sigma x)) pi) (Fimplies (msubst p x id) (msubst q x id))).
-
-Axiom let_equiv : forall (id:ident) (id':ident) (t:term) (f:fmla),
-  forall (sigma:(map mident value)) (pi:(list (ident* value)%type)),
-  (fresh_in_fmla id' f) -> ((eval_fmla sigma pi (Flet id' t (subst f id
-  id'))) -> (eval_fmla sigma pi (Flet id t f))).
-
-Axiom let_equiv2 : forall (id:ident) (id':ident) (t:term) (f:fmla),
-  forall (sigma:(map mident value)) (pi:(list (ident* value)%type)),
-  (fresh_in_fmla id' f) -> ((eval_fmla sigma pi (Flet id' t (subst f id
-  id'))) -> (eval_fmla sigma pi (Flet id t f))).
-
-Axiom let_implies : forall (id:ident) (t:term) (p:fmla) (q:fmla),
-  (valid_fmla (Fimplies p q)) -> (valid_fmla (Fimplies (Flet id t p) (Flet id
-  t q))).
 
 (* Why3 assumption *)
 Fixpoint fresh_in_stmt(id:ident) (s:stmt) {struct s}: Prop :=
@@ -536,11 +555,13 @@ Axiom many_steps_seq : forall (sigma1:(map mident value)) (sigma3:(map mident
   pi2 Sskip n1) /\ ((many_steps sigma2 pi2 s2 sigma3 pi3 Sskip n2) /\
   (n = ((1%Z + n1)%Z + n2)%Z)).
 
-Axiom one_step_change_free : forall (s:stmt) (s':stmt) (sigma:(map mident
-  value)) (sigma':(map mident value)) (pi:(list (ident* value)%type))
-  (pi':(list (ident* value)%type)) (id:ident) (v:value), (fresh_in_stmt id
-  s) -> ((one_step sigma (Cons (id, v) pi) s sigma' pi' s') ->
-  (one_step sigma pi s sigma' pi' s')).
+Axiom type_preservation : forall (s1:stmt) (s2:stmt) (sigma1:(map mident
+  value)) (sigma2:(map mident value)) (pi1:(list (ident* value)%type))
+  (pi2:(list (ident* value)%type)) (sigmat:(map mident datatype)) (pit:(list
+  (ident* datatype)%type)), ((type_stmt sigmat pit s1) /\
+  ((compatible_env sigma1 sigmat pi1 pit) /\ (one_step sigma1 pi1 s1 sigma2
+  pi2 s2))) -> ((type_stmt sigmat pit s2) /\ (compatible_env sigma2 sigmat
+  pi2 pit)).
 
 (* Why3 assumption *)
 Definition valid_triple(p:fmla) (s:stmt) (q:fmla): Prop := forall (sigma:(map
@@ -555,118 +576,40 @@ Definition total_valid_triple(p:fmla) (s:stmt) (q:fmla): Prop :=
   exists pi':(list (ident* value)%type), exists n:Z, (many_steps sigma pi s
   sigma' pi' Sskip n) /\ (eval_fmla sigma' pi' q).
 
-Axiom set1 : forall (a:Type) {a_WT:WhyType a}, Type.
-Parameter set1_WhyType : forall (a:Type) {a_WT:WhyType a}, WhyType (set1 a).
-Existing Instance set1_WhyType.
-
-Parameter mem: forall {a:Type} {a_WT:WhyType a}, a -> (set1 a) -> Prop.
-
 (* Why3 assumption *)
-Definition infix_eqeq {a:Type} {a_WT:WhyType a}(s1:(set1 a)) (s2:(set1
-  a)): Prop := forall (x:a), (mem x s1) <-> (mem x s2).
+Definition assigns(sigma:(map mident value)) (a:(set.Set.set mident))
+  (sigma':(map mident value)): Prop := forall (i:mident), (~ (set.Set.mem i
+  a)) -> ((get sigma i) = (get sigma' i)).
 
-Axiom extensionality : forall {a:Type} {a_WT:WhyType a}, forall (s1:(set1 a))
-  (s2:(set1 a)), (infix_eqeq s1 s2) -> (s1 = s2).
-
-(* Why3 assumption *)
-Definition subset {a:Type} {a_WT:WhyType a}(s1:(set1 a)) (s2:(set1
-  a)): Prop := forall (x:a), (mem x s1) -> (mem x s2).
-
-Axiom subset_trans : forall {a:Type} {a_WT:WhyType a}, forall (s1:(set1 a))
-  (s2:(set1 a)) (s3:(set1 a)), (subset s1 s2) -> ((subset s2 s3) ->
-  (subset s1 s3)).
-
-Parameter empty: forall {a:Type} {a_WT:WhyType a}, (set1 a).
-
-(* Why3 assumption *)
-Definition is_empty {a:Type} {a_WT:WhyType a}(s:(set1 a)): Prop :=
-  forall (x:a), ~ (mem x s).
-
-Axiom empty_def1 : forall {a:Type} {a_WT:WhyType a}, (is_empty (empty :(set1
-  a))).
-
-Parameter add: forall {a:Type} {a_WT:WhyType a}, a -> (set1 a) -> (set1 a).
-
-Axiom add_def1 : forall {a:Type} {a_WT:WhyType a}, forall (x:a) (y:a),
-  forall (s:(set1 a)), (mem x (add y s)) <-> ((x = y) \/ (mem x s)).
-
-Parameter remove: forall {a:Type} {a_WT:WhyType a}, a -> (set1 a) -> (set1
-  a).
-
-Axiom remove_def1 : forall {a:Type} {a_WT:WhyType a}, forall (x:a) (y:a)
-  (s:(set1 a)), (mem x (remove y s)) <-> ((~ (x = y)) /\ (mem x s)).
-
-Axiom subset_remove : forall {a:Type} {a_WT:WhyType a}, forall (x:a) (s:(set1
-  a)), (subset (remove x s) s).
-
-Parameter union: forall {a:Type} {a_WT:WhyType a}, (set1 a) -> (set1 a) ->
-  (set1 a).
-
-Axiom union_def1 : forall {a:Type} {a_WT:WhyType a}, forall (s1:(set1 a))
-  (s2:(set1 a)) (x:a), (mem x (union s1 s2)) <-> ((mem x s1) \/ (mem x s2)).
-
-Parameter inter: forall {a:Type} {a_WT:WhyType a}, (set1 a) -> (set1 a) ->
-  (set1 a).
-
-Axiom inter_def1 : forall {a:Type} {a_WT:WhyType a}, forall (s1:(set1 a))
-  (s2:(set1 a)) (x:a), (mem x (inter s1 s2)) <-> ((mem x s1) /\ (mem x s2)).
-
-Parameter diff: forall {a:Type} {a_WT:WhyType a}, (set1 a) -> (set1 a) ->
-  (set1 a).
-
-Axiom diff_def1 : forall {a:Type} {a_WT:WhyType a}, forall (s1:(set1 a))
-  (s2:(set1 a)) (x:a), (mem x (diff s1 s2)) <-> ((mem x s1) /\ ~ (mem x s2)).
-
-Axiom subset_diff : forall {a:Type} {a_WT:WhyType a}, forall (s1:(set1 a))
-  (s2:(set1 a)), (subset (diff s1 s2) s1).
-
-Parameter choose: forall {a:Type} {a_WT:WhyType a}, (set1 a) -> a.
-
-Axiom choose_def : forall {a:Type} {a_WT:WhyType a}, forall (s:(set1 a)),
-  (~ (is_empty s)) -> (mem (choose s) s).
-
-Parameter all: forall {a:Type} {a_WT:WhyType a}, (set1 a).
-
-Axiom all_def : forall {a:Type} {a_WT:WhyType a}, forall (x:a), (mem x
-  (all :(set1 a))).
-
-(* Why3 assumption *)
-Definition assigns(sigma:(map mident value)) (a:(set1 mident)) (sigma':(map
-  mident value)): Prop := forall (i:mident), (~ (mem i a)) -> ((get sigma
-  i) = (get sigma' i)).
-
-Axiom assigns_refl : forall (sigma:(map mident value)) (a:(set1 mident)),
-  (assigns sigma a sigma).
+Axiom assigns_refl : forall (sigma:(map mident value)) (a:(set.Set.set
+  mident)), (assigns sigma a sigma).
 
 Axiom assigns_trans : forall (sigma1:(map mident value)) (sigma2:(map mident
-  value)) (sigma3:(map mident value)) (a:(set1 mident)), ((assigns sigma1 a
-  sigma2) /\ (assigns sigma2 a sigma3)) -> (assigns sigma1 a sigma3).
+  value)) (sigma3:(map mident value)) (a:(set.Set.set mident)),
+  ((assigns sigma1 a sigma2) /\ (assigns sigma2 a sigma3)) -> (assigns sigma1
+  a sigma3).
 
 Axiom assigns_union_left : forall (sigma:(map mident value)) (sigma':(map
-  mident value)) (s1:(set1 mident)) (s2:(set1 mident)), (assigns sigma s1
-  sigma') -> (assigns sigma (union s1 s2) sigma').
+  mident value)) (s1:(set.Set.set mident)) (s2:(set.Set.set mident)),
+  (assigns sigma s1 sigma') -> (assigns sigma (set.Set.union s1 s2) sigma').
 
 Axiom assigns_union_right : forall (sigma:(map mident value)) (sigma':(map
-  mident value)) (s1:(set1 mident)) (s2:(set1 mident)), (assigns sigma s2
-  sigma') -> (assigns sigma (union s1 s2) sigma').
+  mident value)) (s1:(set.Set.set mident)) (s2:(set.Set.set mident)),
+  (assigns sigma s2 sigma') -> (assigns sigma (set.Set.union s1 s2) sigma').
 
 (* Why3 assumption *)
-Fixpoint stmt_writes(s:stmt) (w:(set1 mident)) {struct s}: Prop :=
+Fixpoint stmt_writes(s:stmt) (w:(set.Set.set mident)) {struct s}: Prop :=
   match s with
   | (Sskip|(Sassert _)) => True
-  | (Sassign id _) => (mem id w)
+  | (Sassign id _) => (set.Set.mem id w)
   | (Sseq s1 s2) => (stmt_writes s1 w) /\ (stmt_writes s2 w)
   | (Sif t s1 s2) => (stmt_writes s1 w) /\ (stmt_writes s2 w)
   | (Swhile _ _ body) => (stmt_writes body w)
   end.
 
-Parameter fresh_from: fmla -> stmt -> ident.
+Parameter fresh_from: fmla -> ident.
 
-Axiom fresh_from_fmla : forall (s:stmt) (f:fmla),
-  (fresh_in_fmla (fresh_from f s) f).
-
-Axiom fresh_from_stmt : forall (s:stmt) (f:fmla),
-  (fresh_in_stmt (fresh_from f s) s).
+Axiom fresh_from_fmla : forall (f:fmla), (fresh_in_fmla (fresh_from f) f).
 
 Parameter abstract_effects: stmt -> fmla -> fmla.
 
@@ -685,8 +628,7 @@ Fixpoint wp(s:stmt) (q:fmla) {struct s}: fmla :=
   | Sskip => q
   | (Sassert f) => (Fand f (Fimplies f q))
   | (Sseq s1 s2) => (wp s1 (wp s2 q))
-  | (Sassign x t) => let id := (fresh_from q s) in (Flet id t (msubst q x
-      id))
+  | (Sassign x t) => let id := (fresh_from q) in (Flet id t (msubst q x id))
   | (Sif t s1 s2) => (Fand (Fimplies (Fterm t) (wp s1 q))
       (Fimplies (Fnot (Fterm t)) (wp s2 q)))
   | (Swhile cond inv body) => (Fand inv (abstract_effects body
@@ -720,10 +662,11 @@ Theorem progress : forall (s:stmt),
   | Sskip => True
   | (Sassign m t) => forall (sigma:(map mident value)) (pi:(list (ident*
       value)%type)) (sigmat:(map mident datatype)) (pit:(list (ident*
-      datatype)%type)) (q:fmla), (type_stmt sigmat pit s) ->
-      ((eval_fmla sigma pi (wp s q)) -> ((~ (s = Sskip)) ->
-      exists sigma':(map mident value), exists pi':(list (ident*
-      value)%type), exists s':stmt, (one_step sigma pi s sigma' pi' s')))
+      datatype)%type)) (q:fmla), (compatible_env sigma sigmat pi pit) ->
+      ((type_stmt sigmat pit s) -> ((eval_fmla sigma pi (wp s q)) ->
+      ((~ (s = Sskip)) -> exists sigma':(map mident value), exists pi':(list
+      (ident* value)%type), exists s':stmt, (one_step sigma pi s sigma' pi'
+      s'))))
   | (Sseq s1 s2) => True
   | (Sif t s1 s2) => True
   | (Sassert f) => True
